To see that a circle has the formula $\sqrt{(x-a)^2+(y-b)^2}=r$ it is sufficient to realize that the left hand side of the expression is nothing else but the Euclidean distance between the point $(x,y)$ and the point $(a,b)$, which is set equal to $r$.

$$
\begin{array}{c}
x^2+y^2+10x-6y+30 = 0 \\
x^2+10x+25 +y^2-6y+9 = 25 + 9 -30 \\
(x+5)^2+(y-3)^2 = 2^2
\end{array}
$$

The center of the circle is $(-5,3)$ and the radius is $2$.

$$
\begin{array}{c}
3x^2+3y^2+18x-24y = -39 \\
x^2+y^2+6x-8y = -13 \\
x^2+6x+9 + y^2-8y+16 = 9+16-13 \\
(x+3)^2+(y-4)^2 = 12
\end{array}
$$

The center of the circle is $(-3,4)$ and the radius is $2\sqrt{3}$.
