Recall that the distance between two points $(x_1,y_1)$ and $(x_2,y_2)$ is given by $\sqrt{(x_1-x_2)^2+(y_1-y_2)^2}$.

1. Distance between $(1, 3)$ and $(2, 4)$ is given by
$\sqrt{(1-2)^2+(3-4)^2} = \sqrt{1+1} = \sqrt{2}$
1. Distance between $(-1, 2)$ and $(3, 3)$ is given by
$\sqrt{(-1-3)^2+(2-3)^2} = \sqrt{(4)^2+(1)^2} = \sqrt{17}$
1. Distance between $(\tfrac{3}{2},-2)$ and $(-5,1)$ is given by
$\sqrt{(\tfrac{3}{2}-(-5))^2+(-2-1)^2} = \sqrt{(\tfrac{13}{2})^2+(3)^2} = \sqrt{(\tfrac{13}{2})^2+(3)^2} = \sqrt{\tfrac{169}{4} + 9} = \sqrt{\tfrac{205}{4}} = \tfrac{\sqrt{205}}{2}$
1. Distance between $(x,y)$ and $(2x,y+3)$ is given by
$\sqrt{(x-2x)^2+(y-(y+3))^2} = \sqrt{x^2+3^2} = \sqrt{x^2+9}$
1. Distance between $(a, b)$ and $(-a, b)$ is given by
$\sqrt{(a-(-a))^2+(b-b)^2} = \sqrt{(2a)^2+0^2} = \sqrt{4a^2} = 2|a|$. We need absolute value because distance is always non-negative.
1. Distance between $(a,3)$ and $(2+a,5)$ is given by
$\sqrt{(a-(2+a))^2+(3-5)^2} = \sqrt{(2)^2+(2)^2} = 2\sqrt{2}$
