**(a)**

The first five terms of the sequence $\left\{\frac{2 n-1}{3 n+2}\right\}_{n \in \mathbb{N}}$ are

$$
\begin{array}{l}
x_{1}=\frac{2(1)-1}{3(1)+2}=\frac{2-1}{3+2}=\frac{1}{5}, \\
x_{2}=\frac{2(2)-1}{3(2)+2}=\frac{4-1}{6+2}=\frac{3}{8}, \\
x_{3}=\frac{2(3)-1}{3(3)+2}=\frac{6-1}{9+2}=\frac{5}{11}, \\
x_{4}=\frac{2(4)-1}{3(4)+2}=\frac{8-1}{12+2}=\frac{7}{14}=\frac{1}{2}, \\
x_{5}=\frac{2(5)-1}{3(5)+2}=\frac{10-1}{15+2}=\frac{9}{17} \text {. }
\end{array}
$$


**(b)**
The first five terms of the sequence $\left\{\frac{1-(-1)^{n}}{n^{3}}\right\}_{n \in \mathbb{N}}$ are

$$
\begin{array}{l}
x_{1}=\frac{1-(-1)^{1}}{1^{3}}=\frac{1-(-1)}{1}=\frac{1+1}{1}=\frac{2}{1}=2, \\
x_{2}=\frac{1-(-1)^{2}}{2^{3}}=\frac{1-(1)}{8}=\frac{1-1}{8}=\frac{0}{8}=0, \\
x_{3}=\frac{1-(-1)^{3}}{3^{3}}=\frac{1-(-1)}{27}=\frac{1+1}{27}=\frac{2}{27}, \\
x_{4}=\frac{1-(-1)^{4}}{4^{3}}=\frac{1-(1)}{64}=\frac{1-1}{64}=\frac{0}{64}=0, \\
x_{5}=\frac{1-(-1)^{5}}{5^{3}}=\frac{1-(-1)}{125}=\frac{1+1}{125}=\frac{2}{125} .
\end{array}
$$

**(c)**
The first five terms of the sequence $\left\{\frac{(-1)^{n-1}}{(2)(4)(6) \cdots(2 n)}\right\}_{n \in \mathbb{N}}$ are

$$
\begin{array}{l}
x_{1}=\frac{(-1)^{1-1}}{(2)}=\frac{(-1)^{0}}{2}=\frac{1}{2}, \\
x_{2}=\frac{(-1)^{2-1}}{(2)(4)}=\frac{(-1)^{1}}{8}=\frac{-1}{8} \\
x_{3}=\frac{(-1)^{3-1}}{(2)(4)(6)}=\frac{(-1)^{2}}{48}=\frac{1}{(48)}, \\
x_{4}=\frac{(-1)^{4-1}}{(2)(4)(6)(8)}=\frac{(-1)^{3}}{384}=\frac{-1}{384}, \\
x_{5}=\frac{(-1)^{5-1}}{(2)(4)(6)(8)(10)}=\frac{(-1)^{4}}{3,840}=\frac{1}{(3,840)}
\end{array}
$$


**(d)**

The first five terms of the sequence $\left\{\frac{1}{2}+\frac{1}{4}+\frac{1}{8}+\cdots+\frac{1}{2^{n}}\right\}_{n \in \mathbb{N}}$ are

$$
\begin{array}{l}
x_{1}=\sum_{i=1}^{1} \frac{1}{2^{i}}=\frac{1}{2^{1}}=\frac{1}{2}, \\
x_{2}=\sum_{i=1}^{2} \frac{1}{2^{i}}=\frac{1}{2^{1}}+\frac{1}{2^{2}}=\frac{1}{2}+\frac{1}{4}=\frac{3}{4} \\
x_{3}=\sum_{i=1}^{3} \frac{1}{2^{i}}=\frac{1}{2^{1}}+\frac{1}{2^{2}}+\frac{1}{2^{3}}=\frac{1}{2}+\frac{1}{4}+\frac{1}{8}=\frac{3}{4}+\frac{1}{8}=\frac{7}{8}, \\
x_{4}=\sum_{i=1}^{4} \frac{1}{2^{i}}=\frac{1}{2^{1}}+\frac{1}{2^{2}}+\frac{1}{2^{3}}+\frac{1}{2^{4}}=\frac{1}{2}+\frac{1}{4}+\frac{1}{8}+\frac{1}{16}=\frac{7}{8}+\frac{1}{16}=\frac{15}{16}, \\
x_{5}=\sum_{i=1}^{5} \frac{1}{2^{i}}=\frac{1}{2^{1}}+\frac{1}{2^{2}}+\frac{1}{2^{3}}+\frac{1}{2^{4}}=\frac{1}{2}+\frac{1}{4}+\frac{1}{8}+\frac{1}{16}+\frac{1}{32}=\frac{15}{16}+\frac{1}{32}=\frac{31}{32} .
\end{array}
$$


**(e)**

The first five terms of the sequence $\left\{\frac{(-1)^{n-1} x^{2 n-1}}{(2 n-1) !}\right\}_{n \in \mathbb{N}}$ are

$$
\begin{array}{l}
x_{1}=\frac{(-1)^{1-1} x^{2(1)-1}}{(2(1)-1) !}=\frac{(-1)^{0} x^{2-1}}{((2-1) !}=\frac{(1) x^{1}}{1 !}=\frac{x^{1}}{1}=x, \\
x_{2}=\frac{(-1)^{2-1} x^{2(2)-1}}{(2(2)-1) !}=\frac{(-1)^{1} x^{4-1}}{((4-1) !}=\frac{(-1) x^{3}}{3 !}=\frac{-x^{3}}{(3)(2)(1)}=\frac{-x^{3}}{6}, \\
x_{3}=\frac{(-1)^{3-1} x^{2(3)-1}}{(2(3)-1) !}=\frac{(-1)^{2} x^{6-1}}{((6-1) !}=\frac{(1) x^{5}}{5 !}=\frac{x^{5}}{(5)(4)(3)(2)(1)}=\frac{x^{5}}{120}, \\
x_{4}=\frac{(-1)^{4-1} x^{2(4)-1}}{(2(4)-1) !}=\frac{(-1)^{3} x^{8-1}}{((8-1) !}=\frac{(-1) x^{7}}{7 !}=\frac{-x^{7}}{(7)(6)(5)(4)(3)(2)(1)}=\frac{-x^{7}}{5,040}, \\
x_{5}=\frac{(-1)^{5-1} x^{2(5)-1}}{(2(5)-1) !}=\frac{(-1)^{4} x^{10-1}}{((10-1) !}=\frac{(1) x^{9}}{9 !}=\frac{x^{9}}{(9)(8)(7)(6)(5)(4)(3)(2)(1)}=\frac{x^{9}}{362,880}
\end{array}
$$
