Consider the geometric progression

$$
\left\{P_{n}\right\}_{n=1}^{\infty}=\left\{a, a r, a r^{2}, \cdots\right\}=\left\{a r^{(n-1)}\right\}_{n=1}^{\infty},
$$

where $r \notin\{0,1\}$. Note that the sum of the first $N$ terms of this geometric progression is defined by

$$
S_{N}=\sum_{n=1}^{N} P_{n}=\sum_{n=1}^{N} a r^{(n-1)}=\sum_{k=0}^{N-1} a r^{k}
$$

Use the principle of mathematical induction to prove that this partial sum for this arbitrary geometric progression is given by the formula

$$
S_{N}=\frac{a\left(1-r^{N}\right)}{(1-r)}
$$
