**(a)**

$$
\begin{array}{ll}
\frac{\mathrm{dy}}{\mathrm{dx}}&=\frac{\mathrm{df}}{\mathrm{dx}} \mathrm{g}(\mathrm{x})+\frac{\mathrm{dg}}{\mathrm{dx}} \mathrm{f}(\mathrm{x}) \\
&=3 x^{2}\left(x^{2}+4\right)+(2 x+0) x^{3}\\
&=3 x^{4}+12 x^{2}+2 x^{4} \\
&=5 x^{4}+12 x^{2}
\end{array}
$$

**(b)**

$$
\begin{array}{ll}
\frac{d y}{d x}&=\frac{d f}{d x} g(x)+\frac{d g}{d x} f(x) \\
& =(1)\left(x^{2}-5 x+7\right)+(2 x-5(1)+0)(x-3) \\
& =x^{2}-5 x+7+2 x^{2}-6 x-5 x+15 \\
& =3 x^{2}-16 x+22
\end{array}
$$

**(c)**

$$
\begin{array}{ll}
\frac{d y}{d x}&=\frac{\frac{d f}{d x} g(x)-\frac{d g}{d x} f(x)}{[g(x)]^{2}} \\
\frac{d y}{d x} & =\frac{d}{d x}\left\{\frac{\left(x^{3}+6 x^{2}-2\right)}{x^{4}}\right\} \\
& =\frac{d}{d x}\left\{\left(x^{3}+6 x^{2}-2\right) x^{-4}\right\} \\
& =\left(\frac{d\left(x^{3}+6 x^{2}-2\right)}{d x}\right) x^{-4}+\left(\frac{d x^{-4}}{d x}\right)\left(x^{3}+6 x^{2}-2\right) \\
& =\left(3 x^{2}+12 x\right) x^{-4}+\left(-4 x^{-5}\right)\left(x^{3}+6 x^{2}-2\right) \\
& =3 x^{-2}+12 x^{-3}-4 x^{-2}-24 x^{-3}+8 x^{-5} \\
& =-x^{-2}-12 x^{-3}+8 x^{-5} .
\end{array}
$$

**(d)**

$$
\begin{array}{ll}
\frac{d y}{d x}&=\frac{\frac{d f}{d x} g(x)-\frac{d g}{d x} f(x)}{[g(x)]^{2}} \\
&=\frac{\left(4 x^{3}+3(1)\right) x^{6}-6 x^{5}\left(x^{4}+3 x\right)}{\left(x^{6}\right)^{2}}\\
& =\frac{4 x^{9}+3 x^{6}-6 x^{9}-18 x^{6}}{x^{12}} \\
& =\frac{-2 x^{9}-15 x^{6}}{x^{12}} \\
& =-2 x^{-3}-15 x^{-6}
\end{array}
$$

**(e)**

$$
\frac{d y}{d x}=0+\frac{d f}{d x} g(x)+\frac{d g}{d x} f(x)
=1 \cdot e^{x}+e^{x} \cdot x
=e^{x}(1+x)
$$


(f) In this example the product rule is used to find the derivative of both terms on the RHS

$$
\begin{array}{ll}
\frac{d y}{d x} & =\left[(2 x) e^{x}+\left(e^{x}\right) x^{2}\right]+\left[(1) \ln x+x \cdot \frac{1}{x}\right] \\
& =2 x e^{x}+x^{2} e^{x}+\ln x+1
\end{array}
$$

**(g)**

$$
\begin{array}{ll}
\frac{dy}{dx}&=\frac{\mathrm{df}}{\mathrm{dx}} \mathrm{g}(\mathrm{x})+\frac{\mathrm{dg}}{\mathrm{dx}} \mathrm{f}(\mathrm{x})\\
& =2 x(1.1)^{x}+\ln (1.1)(1.1)^{x} x^{2} \\
& =(1.1)^{x}\left(2 x+0.0953 x^{2}\right)
\end{array}
$$


**(h)**

$$
\begin{array}{ll}
\frac{dy}{dx}&=\frac{\mathrm{df}}{\mathrm{dx}} \mathrm{g}(\mathrm{x})+\frac{\mathrm{dg}}{\mathrm{dx}} \mathrm{f}(\mathrm{x})\\
&=5 \cdot \mathrm{e}^{\mathrm{x}} \ln \mathrm{x}+5 \frac{1}{\mathrm{x}} \mathrm{e}^{\mathrm{x}}\\
&=5 \cdot \mathrm{e}^{\mathrm{x}}\left(\ln \mathrm{x}+\frac{1}{\mathrm{x}}\right)
\end{array}
$$



**(i)**

$$
\begin{array}{ll}
\frac{d y}{d x}&=\frac{d f}{d x} g(x)+\frac{d g}{d x} f(x)\\
& =\left(3 x^{2}+0\right)(1.2)^{x}+(\ln 1.2)(1.2)^{x}\left(x^{3}+2\right) \\
& =(1.2)^{x}\left[3 x^{2}+0.1823\left(x^{3}+2\right)\right] \\
& =(1.2)^{x}\left[0.1823 x^{3}+3 x^{2}+0.3646\right]
\end{array}
$$

**(j)**

$$
\begin{array}{ll}
\frac{d y}{d x}&=\frac{d f}{d x} g(x)+\frac{d g}{d x}(x)\\
&=-\frac{5}{6} x^{-11 / 6} e^{x}+e^{x} x^{-5 / 6}\\
&=e^{x}\left(x^{-5 / 6}-\frac{5}{6} x^{-11 / 6}\right)
\end{array}
$$

