Use either the product rule or the quotient rule to find the first derivative of each of the following functions.

(a) $y=x^{3}\left(x^{2}+4\right)$;

(b) $y=(x-3)\left(x^{2}-5 x+7\right)$;

(c) $y=\frac{\left(x^{3}+6 x^{2}-2\right)}{x^{4}}$;

(d) $y=\left(x^{4}+3 x\right) x^{-6}$;

(e) $y=5+x e^{x}$;

(f) $y=x^{2} e^{x}+x \ln (x)$;

(g) $y=x^{2}(1.1)^{x}$;

(h) $y=5 e^{x} \ln (x)$;

(i) $y=\left(x^{3}+2\right)(1.2)^{x}$; and

(j) $y=x^{-\left(\frac{5}{6}\right)} e^{x}$.

{cite:ps}`shannon1995`, p. 401