1. Factorizing the LHS

$$
\begin{array}{l}
x^3-4x = 0 \\
x(x^2-4) = 0 \\
x(x-2)(x+2) = 0 \\
x_1 = 0 \quad x_2 = 2 \quad x_3 = -2
\end{array}
$$

2. Making a substitution $y=x^2$, and using Viète's formulas

$$
\begin{array}{l}
x^4 - 5x^2 +4 =0 \\
y^2 - 5y +4 =0 \\
(y-4)(y-1) = 0 \\
y_1 = 4 \quad y_2 = 1 \\
x = \pm 2 \quad \text{or} \quad x = \pm 1 \\
\text{Full solution: }x_1 = -2 \quad x_2 = 2 \quad x_3 = -1 \quad x_4 = 1
\end{array}
$$

3. Making a substitution $y=1/x$, and using Viète's formulas

$$
\begin{array}{l}
x^{-2}-2x^{-1} -15=0 \\
y^2-2y -15=0 \\
(y-5)(y+3) = 0 \\
1/x = 5 \quad \text{or} \quad 1/x = -3 \\
\text{Full solution: }x_1 = -1/5 \quad x_2 = -1/3
\end{array}
$$