1. Completing the square

$$
\begin{array}{l}
x^2 - 5x + 6 = 0 \\
x^2 - 2x\cdot\tfrac{5}{2} + \left(\tfrac{5}{2}\right)^2 + 6 - \tfrac{25}{4}= 0 \\
\left(x - \tfrac{5}{2}\right)^2 = \tfrac{25}{4} - 6 \\
x - \tfrac{5}{2} = \pm \sqrt{\tfrac{1}{4}} \\
x = \tfrac{5 \pm 1}{2}
\end{array}
$$

2. Using Vi√®te's formulas to factor

$$
\begin{array}{l}
y^2 - y - 12 = 0 \\
(y-4)(y+3) = 0 \\
y = 4 \quad \text{or} \quad y = -3 
\end{array}
$$

3. Completing the square

$$
\begin{array}{l}
2x^2 + 60x +800 = 0 \\
x^2 + 30x + 400 = 0 \\
x^2 + 2x\cdot 15 + 225 +400 - 225 = 0 \\
(x+15)^2 = 225 - 400 \\
(x+15)^2 = - 175
\end{array}
$$

The equation has no real roots (it's ok not to give complex solutions).

4. Completing the square

$$
\begin{array}{l}
-\tfrac{1}{4}x^2 + \tfrac{1}{2}x + \tfrac{1}{2} = 0 \\
x^2 - 2x -2 = 0 \\
x^2 - 2x +1 -2-1 = 0 \\
(x-1)^2 = 3 \\
x-1 = \pm \sqrt{3} \\
x = 1 \pm \sqrt{3}
\end{array}
$$

5. Completing the square

$$
\begin{array}{l}
m(m-5) - 3 = 0 \\
m^2 -5m - 3 = 0 \\
m^2 - 2m\cdot\tfrac{5}{2} + \left(\tfrac{5}{2}\right)^2 - 3 - \tfrac{25}{4} = 0 \\
\left(m-\tfrac{5}{2}\right)^2 = 3+\tfrac{25}{4} \\
m-\tfrac{5}{2} = \pm \sqrt{\tfrac{37}{4}} \\
m = \tfrac{5}{2} \pm \sqrt{\tfrac{37}{4}} \\
m = \tfrac{5\pm \sqrt{37}}{2}
\end{array}
$$

6. Completing the square

$$
\begin{array}{l}
0.1 p^2 +p -2.4 = 0 \\
p^2 + 10p -24 = 0 \\
p^2 + 2p\cdot 5 + 25 - 24 -25 = 0 \\
(p+5)^2 = 49 \\
p+5 = \pm 7 \\
p = -5 \pm 7
\end{array}
$$
