**3(a)**

The utility function is

$$
U(x, y)=x+\sqrt{y}=x+y^{\frac{1}{2}}
$$

The marginal utility of commodity $x$ is

$$
M U_{x}(x, y)=\frac{\partial U(x, y)}{\partial x}=1
$$

The marginal utility of commodity $y$ is

$$
M U_{y}(x, y)=\frac{\partial U(x, y)}{\partial y}=\left(\frac{1}{2}\right) y^{-\left(\frac{1}{2}\right)}=\frac{1}{2 \sqrt{y}}
$$

The marginal rate of substitution of commodity $x$ for commodity $y$ is

$$
M R S_{x, y}(x, y)=\frac{M U_{x}(x, y)}{M U_{y}(x, y)}=\frac{1}{\left(\frac{1}{2 \sqrt{y}}\right)}=2 \sqrt{y}
$$



**3(b)**

The utility function is

$$
U(x, y)=x+\ln y
$$

The marginal utility of commodity $x$ is

$$
M U_{x}(x, y)=\frac{\partial U(x, y)}{\partial x}=1
$$

The marginal utility of commodity $y$ is

$$
M U_{y}(x, y)=\frac{\partial U(x, y)}{\partial y}=\frac{1}{y}
$$

The marginal rate of substitution of commodity $x$ for commodity $y$ is

$$
M R S_{x, y}(x, y)=\frac{M U_{x}(x, y)}{M U_{y}(x, y)}=\frac{1}{\left(\frac{1}{y}\right)}=y
$$




**3(c)**

The utility function is

$$
U(x, y)=\left(x-x_{0}\right)^{\alpha}\left(y-y_{0}\right)^{1-\alpha}
$$

The marginal utility of commodity $x$ is

$$
M U_{x}(x, y)=\frac{\partial U(x, y)}{\partial x}=\alpha\left(x-x_{0}\right)^{\alpha-1}\left(y-y_{0}\right)^{1-\alpha}
$$

The marginal utility of commodity $y$ is

$$
\begin{array}{ll}
M U_{y}(x, y) &= \frac{\partial U(x, y)}{\partial y}=(1-\alpha)\left(x-x_{0}\right)^{\alpha}\left(y-y_{0}\right)^{1-\alpha-1} \\
& =(1-\alpha)\left(x-x_{0}\right)^{\alpha}\left(y-y_{0}\right)^{-\alpha}
\end{array}
$$

The marginal rate of substitution of commodity $x$ for commodity $y$ is

$$
\begin{array}{c}
M R S_{x, y}(x, y)=\frac{M U_{x}(x, y)}{M U_{y}(x, y)}=\frac{\alpha\left(x-x_{0}\right)^{\alpha-1}\left(y-y_{0}\right)^{1-\alpha}}{(1-\alpha)\left(x-x_{0}\right)^{\alpha}\left(y-y_{0}\right)^{-\alpha}} \\
=\frac{\alpha\left(y-y_{0}\right)}{(1-\alpha)\left(x-x_{0}\right)}
\end{array}
$$



**3(d)**

The utility function is

$$
U(x, y)=\left(\alpha x^{\rho}+\beta y^{\rho}\right)^{\frac{1}{\rho}}
$$

The marginal utility of commodity $x$ is

$$
\begin{array}{c}
M U_{x}(x, y)=\frac{\partial U(x, y)}{\partial x}=\left(\frac{1}{\rho}\right)\left(\alpha x^{\rho}+\beta y^{\rho}\right)^{\left(\frac{1}{\rho}\right)-1} \rho \alpha x^{\rho-1} \\
=\alpha x^{\rho-1}\left(\alpha x^{\rho}+\beta y^{\rho}\right)^{\left(\frac{1}{\rho}\right)-1}=\alpha x^{\rho-1}\left(\alpha x^{\rho}+\beta y^{\rho}\right)^{\frac{1-\rho}{\rho}}
\end{array}
$$

The marginal utility of commodity $y$ is

$$
\begin{array}{ll}
M U_{y}(x, y)&=\frac{\partial U(x, y)}{\partial y} \\ 
&=\left(\frac{1}{\rho}\right)\left(\alpha x^{\rho}+\beta y^{\rho}\right)^{\left(\frac{1}{\rho}\right)-1} \rho \beta y^{\rho-1} \\
& =\beta y^{\rho-1}\left(\alpha x^{\rho}+\beta y^{\rho}\right)^{\left(\frac{1}{\rho}\right)-1}\\
&=\beta y^{\rho-1}\left(\alpha x^{\rho}+\beta y^{\rho}\right)^{\frac{1-\rho}{\rho}}\\
\end{array}
$$

The marginal rate of substitution of commodity $x$ for commodity $y$ is

$$
\begin{array}{c}
M R S_{x, y}(x, y)=\frac{M U_{x}(x, y)}{M U_{y}(x, y)}=\frac{\alpha x^{\rho-1}\left(\alpha x^{\rho}+\beta y^{\rho}\right)^{\frac{1-\rho}{\rho}}}{\beta y^{\rho-1}\left(\alpha x^{\rho}+\beta y^{\rho}\right)^{\frac{1-\rho}{\rho}}} \\
=\frac{\alpha x^{\rho-1}}{\beta y^{\rho-1}}=\frac{\alpha y^{1-\rho}}{\beta x^{1-\rho}}=\left(\frac{\alpha}{\beta}\right)\left(\frac{y}{x}\right)^{1-\rho}
\end{array}
$$
