**(a)**

$C'(x) = 3x + 4$ and $C(0) = 40$

$$
\begin{array}{ll}
C(x) &= \int (3x + 4) \mathop{dx} \\
&= \frac{3}{2}x^2 + 4x + C
\end{array}
$$

$C(0) = 40 \iff \frac{3}{2}(0)^2 + 4(0) + C = 40 \iff C = 40$

Therefore $C(x) = \frac{3}{2}x^2 + 4x + 40$.


**(b)**

$C'(x) = ax + b$ and $C(0) = C_0$

$$
\begin{array}{ll}
C(x) &= \int (ax + b) \mathop{dx} \\
&= \frac{a}{2}x^2 + bx + C
\end{array}
$$

$C(0) = C_0 \iff \frac{a}{2}(0)^2 + b(0) + C = C_0 \iff C = C_0$

Therefore $C(x) = \frac{a}{2}x^2 + bx + C_0$.

*Source: SHSC Exercise 9.1.2, page 324*
