Given: $f''(x) = x^2$.

Then $f'(x) = \int x^2 \mathop{dx} = \frac{1}{3} x^3 + A$, where $A$ is an arbitrary constant.

Then $f(x) = \int \frac{1}{3} x^3 + A \mathop{dx} = \frac{1}{12} x^4 + Ax + B$, where $A$ and $B$ are arbitrary constants. 
This is the general form of the function whose second derivative is $x^2$.

We also know $f'(0) = -1 \iff \frac{1}{3} (0) + A = -1 \iff A = -1$, and $f(0) = 1 \iff B = 1$ by the same logic.

Therefore in this case $f(x) = \frac{1}{12} x^4 - x + 1$.

*Source: SHSC Exercise 9.1.10, page 325*
