(a)

$$
\frac{\partial Y}{\partial K} 
= (0.06157)(1.356)K^{1.356 - 1} S^{0.562}
= 0.08348892 K^{0.356} S^{0.562}
$$


$$
\frac{\partial Y}{\partial S}
= (0.06157)(0.562) K^{1.356} S^{0.562 - 1}
= 0.03460234 K^{1.356} S^{-0.438}
$$

(b)

$$
\begin{array}{ll}
Y(2K, 2S) &= 0.06157 (2K)^{1.356} (2S)^{0.562} \\
&= (0.06157)(2)^{1.356} (2)^{0.562} K^{1.356} S^{0.562} \\
&= (0.06157)(2)^{1.356 + 0.562} K^{1.356} S^{0.562} \\
&= (2)^{1.356 + 0.562} Y(K, S) \\
&\approx 0.23267 K^{1.356} S^{0.562}
\end{array}
$$

In other words, the size of the catch increases by a factor of $(2)^{1.356 + 0.562} \approx 3.779$ when both inputs are scaled by a factor of two.
