**(a)**

$$\frac{\partial U}{\partial X}=10\left(0.6 X^{-0.4}\right) L^{0.5}=0.6 \frac{U}{X}=6 X^{-0.4} L^{0.5}$$
$$\frac{\partial \mathrm{U}}{\partial \mathrm{L}}=10 \mathrm{X}^{0.6}\left(0.5 \mathrm{~L}^{-0.5}\right)=0.5 \frac{\mathrm{U}}{\mathrm{L}}=5 \mathrm{X}^{0.6} \mathrm{~L}^{-0.5}$$

$$\frac{\partial^{2} U}{\partial X^{2}}=6\left(-0.4 X^{-1.4}\right) L^{0.5}=-2.4 X_{1}^{-1.4} L^{0.5}$$

$$\frac{\partial^{2} U}{\partial L^{2}} \quad=5 X^{0.6}\left(-0.5 L^{-1.5}\right)=-2.5 X_{1}^{0.6} L^{-1.5}$$

$$\frac{\partial^{2} \mathrm{U}}{\partial \mathrm{X} \partial \mathrm{L}}=6 \mathrm{X}^{-0.4}\left(0.5 \mathrm{~L}^{-0.5}\right)=3 \mathrm{X}_{1}^{-0.4} \mathrm{~L}^{-0.5}$$



**(b)**

$$\frac{\partial \mathrm{C}}{\partial \mathrm{Y}}=50\left(0.8 \mathrm{Y}^{-0.2}\right) \mathrm{i}^{0.3}=0.8 \frac{\mathrm{C}}{\mathrm{Y}}=40 \mathrm{Y}^{-0.2} \mathrm{i}^{0.3}$$

$$
\frac{\partial C}{\partial \mathrm{i}}= 50 \mathrm{Y}^{0.8}\left(0.3 \mathrm{i}^{-0.7}\right)=0.3 \frac{\mathrm{C}}{\mathrm{i}}=15 \mathrm{Y}^{-0.8} \mathrm{i}^{-0.7}
$$

$$\frac{\partial^{2} \mathrm{C}}{\partial \mathrm{Y} \partial \mathrm{i}} \quad=40 \mathrm{Y}^{-0.2}\left(0.3 \mathrm{i}^{-0.7}\right)=12 \mathrm{Y}^{-0.2} \mathrm{i}^{-0.7}$$

$$\frac{\partial^{2} \mathrm{C}}{\partial \mathrm{Y}^{2}}=40\left(-0.2 \mathrm{Y}^{-1.2}\right) \mathrm{i}^{0.3}=-8 \mathrm{Y}^{-1.2} \mathrm{i}^{0.3}$$

$$\frac{\partial^{2} \mathrm{C}}{\partial \mathrm{i}^{2}} \quad=15 \mathrm{Y}^{0.8}\left(-0.7 \mathrm{i}^{-1.7}\right)=-10.5 \mathrm{Y}^{0.8} \mathrm{i}^{-1.7}$$






**(c)**

$$\frac{\partial C}{\partial Y}=0+2\left(0.9 Y^{-0.1}\right)+0=1.8 Y^{-0.1}$$

$$
\frac{\partial C}{\partial \mathrm{i}}=0+0+5\left(0.5 \mathrm{i}^{-0.5}\right)=2.5 \mathrm{i}^{-0.5}
$$

$$\frac{\partial^{2} C}{\partial Y \partial i}=0$$

$$
\frac{\partial^{2} \mathrm{C}}{\partial \mathrm{Y}^{2}}=1.8\left(-0.1 \mathrm{Y}^{-1.1}\right)=-0.18 \mathrm{Y}^{-1.1} \\
\frac{\partial^{2} \mathrm{C}}{\partial \mathrm{i}^{2}}=2.5\left(-0.5 \mathrm{i}^{-1.5}\right)=-1.25 \mathrm{i}^{-1.5}
$$





**(d)**

$$\frac{\partial(\mathrm{TC})}{\partial \mathrm{X}_{1}}=0+5(1)+0-2(1) \sqrt{\mathrm{X}_{2}}=5-2 \sqrt{\mathrm{X}_{2}}$$

$$
\frac{\partial(\mathrm{TC})}{\partial \mathrm{X}_{2}}=0+0+6(1)-0.2 \mathrm{X}_{1}\left(0.5 \mathrm{X}_{2}^{-0.5}\right)=6-0.1 \mathrm{X}_{1} \mathrm{X}_{2}^{-0.5}
$$

$$\frac{\partial^{2}(\mathrm{TC})}{\partial \mathrm{X}_{1} \partial \mathrm{X}_{2}}=0-0.2\left(0.5 \mathrm{X}_{2}^{-0.5}\right)=-0.1 \mathrm{X}_{2}^{-0.5}$$

$$\frac{\partial^{2}(\mathrm{TC})}{\partial \mathrm{X}_{1}{ }^{2}}=0$$

$$\frac{\partial^{2}(\mathrm{TC})}{\partial \mathrm{X}_{2}^{2}}=0-0.1 \mathrm{X}_{1}\left(-0.5 \mathrm{X}_{2}^{-1.5}\right)=0.05 \mathrm{X}_{1} \mathrm{X}_{2}^{-1.5}$$





**(e)**

$$\frac{\partial \mathrm{U}}{\partial \mathrm{X}_{1}}=5 \frac{1}{\mathrm{X}_{1}}+0=5 \frac{1}{\mathrm{X}_{1}}$$

$$\frac{\partial U}{\partial X_{2}}=0+2 \frac{1}{X_{2}}=2 \frac{1}{X_{2}}$$

$$\frac{\partial^{2} \mathrm{U}}{\partial \mathrm{X}_{1}^{2}}=-0.5 \mathrm{X}_{1}^{-2}$$

$$
\frac{\partial^{2} U}{\partial X_{2}^{2}}=-2 X_{2}^{-2}
$$




**(f)**

$$\frac{\partial \mathrm{Q}}{\partial \mathrm{K}}=50\left(0.7 \mathrm{~K}^{-0.3}\right) \mathrm{L}^{0.3}=0.7 \frac{\mathrm{Q}}{\mathrm{K}}=35 \mathrm{~K}^{-0.3} \mathrm{~L}^{0.3}$$

$$\frac{\partial \mathrm{Q}}{\partial \mathrm{L}}=50 \mathrm{~K}^{-0.7}\left(0.3 \mathrm{~L}^{-0.7}\right)=0.3 \frac{\mathrm{Q}}{\mathrm{L}}=15 \mathrm{~K}^{0.7} \mathrm{~L}^{-0.7}$$

$$\frac{\partial^{2} \mathrm{Q}}{\partial \mathrm{K}^{2}} \quad=35\left(-0.3 \mathrm{~K}^{-1.3} \mathrm{~L}^{0.3}\right)=-10.5 \mathrm{~K}^{-1.3} \mathrm{~L}^{0.3}$$

$$
\frac{\partial^{2} \mathrm{Q}}{\partial \mathrm{L}^{2}} \quad=15 \mathrm{~K}^{-0.7}\left(-0.7 \mathrm{~L}^{-1.7}\right)=-10.5 \mathrm{~K}^{-0.7} \mathrm{~L}^{-1.7}
$$

$$
\frac{\partial^{2} \mathrm{Q}}{\partial \mathrm{K} \partial \mathrm{L}}=35 \mathrm{~K}^{-0.3}\left(0.3 \mathrm{~L}^{-0.7}\right)=10.5 \mathrm{~K}^{-0.3} \mathrm{~L}^{-0.7}
$$




**(g)**

$$\frac{\partial \mathrm{Q}}{\partial \mathrm{K}}=\mathrm{A}\left(\alpha \mathrm{K}^{\alpha-1}\right) \mathrm{L}^{1-\alpha}=\alpha \frac{\mathrm{Q}}{\mathrm{K}}=\alpha \mathrm{AK}^{-(1-\alpha)} \mathrm{L}^{1-\alpha}$$

$$\frac{\partial \mathrm{Q}}{\partial \mathrm{L}}=\mathrm{AK}^{\alpha}(1-\alpha) \mathrm{L}^{1-\alpha-1}=(1-\alpha) \frac{\mathrm{Q}}{\mathrm{L}}=(1-\alpha) \mathrm{AK}^{\alpha} \mathrm{L}^{-\alpha}$$

$$\frac{\partial^{2} \mathrm{Q}}{\partial \mathrm{K}^{2}}=\mathrm{A} \alpha(\alpha-1) \mathrm{K}^{\alpha-1-1} \mathrm{~L}^{1-\alpha}
=\mathrm{A} \alpha(\alpha-1) \mathrm{K}^{\alpha-2} \mathrm{~L}^{1-\alpha}
=\alpha(\alpha-1) \frac{\mathrm{Q}}{\mathrm{K}^{2}}
$$

$$\frac{\partial^{2} \mathrm{Q}}{\partial \mathrm{L}^{2}}=\mathrm{AK}^{\alpha}(1-\alpha)\left(-\alpha \mathrm{L}^{-\alpha-1}\right)
=-\mathrm{A} \alpha(1-\alpha) \mathrm{K}^{\alpha} \mathrm{L}^{-(\alpha+1)}
=-\alpha(1-\alpha) \frac{\mathrm{Q}}{\mathrm{L}^{2}}
$$





**(h)**

$$\frac{\partial q_{1}}{\partial p_{1}}=100\left(-0.6 p_{1}{ }^{-1.6} p_{2}^{0.4} Y^{0.5}\right)=-0.6 \frac{q_{1}}{p_{1}}=-60 p_{1}^{-1.6} p_{2}^{0.4} Y^{0.5}$$

$$\frac{\partial q_{1}}{\partial p_{2}}=100 p_{1}^{-0.6}\left(0.4 p_{2}^{-0.6}\right) Y^{0.5}=0.4 \frac{q_{1}}{p_{2}}=40 p_{1}^{-0.6} p_{2}^{-0.6} Y^{0.5}$$

$$\frac{\partial q_{1}}{\partial Y}=100 p_{1}^{-0.6} \mathrm{p}_{2}^{0.4}\left(0.5 Y^{-0.5}\right)=0.5 \frac{q_{1}}{Y}=50 p_{1}^{-0.6} p_{2}^{0.4} Y^{-0.5}$$

$$\frac{\partial^{2} q_{1}}{\partial p_{1} \partial p_{2}}=-60 p_{1}^{-1.6}\left(0.4 p_{2}^{-0.6}\right) \sqrt{Y}=-24 p_{1}^{-1.6} p_{2}^{-0.6} \sqrt{Y}$$




**(i)**

$$\frac{\partial \mathrm{q}_{2}}{\partial \mathrm{p}_{1}}=50\left(-0.3 \mathrm{p}_{1}^{-1.3}\right) \mathrm{p}_{2}^{-0.5}=-0.3 \frac{\mathrm{q}_{2}}{\mathrm{p}_{1}}=-15 \mathrm{p}_{1}^{-1.3} \mathrm{p}_{2}^{-0.5}$$

$$\frac{\partial q_{2}}{\partial p_{2}}=50 p_{1}^{-0.3}\left(-0.5 p_{2}^{-1.5}\right)=0.5 \frac{q_{2}}{p_{2}}=-25 p_{1}^{-0.3} p_{2}^{-1.5}$$

$$\frac{\partial^{2} \mathrm{q}_{2}}{\partial \mathrm{p}_{1}^{2}}= -15\left(-1.3 \mathrm{p}_{1}{ }^{-2.3}\right) \mathrm{p}_{2}^{-0.5}=19.5 \mathrm{p}_{1}^{-2.3} \mathrm{p}_{2}^{-0.5}$$

$$
\frac{\partial^{2} \mathrm{q}_{2}}{\partial \mathrm{p}_{2}^{2}}=-25 \mathrm{p}_{1}^{-0.3}\left(-1.5 \mathrm{p}_{2}^{-2.5}\right)=37.5 \mathrm{p}_{1}^{-0.3} \mathrm{p}_{2}^{-2.5}
$$




**(j)**

$$\frac{\partial \Pi}{\partial q_{1}}=0+20\left(2 q_{1}\right)+0-8(1)-5(1) q_{2}=40 q_{1}-8-5 q_{2}$$

$$\frac{\partial \Pi}{\partial q_{2}}=0+0+5\left(2 q_{2}\right)-0-5 q_{1}(1)=10 q_{2}-5 q$$

$$\frac{\partial^{2} \Pi}{\partial q_{1}^{2}}=40(1)-0-0=40$$

$$
\frac{\partial^{2} \Pi}{\partial \mathrm{q}_{2}^{2}}=10(1)-0=10
$$

$$
\frac{\partial^{2} \Pi}{\partial q_{1} \partial q_{2}}=0-0-5(1)=5
$$

