(a)

$$
\begin{array}{ll}
El_x z &= \frac{x}{z} \frac{\partial z}{\partial x} \\
&= \frac{x}{z} (3x^{2} y^{-4}) \\
&= 3x^{3} y^{-4} z^{-1} \\
&= 3 \frac{x^{3} y^{-4}}{x^{3} y^{-4}} \\
&= 3
\end{array}
$$

$$
\begin{array}{ll}
El_y z &= \frac{y}{z} \frac{\partial z}{\partial y} \\
&= \frac{y}{z} (-4x^{3} y^{-5}) \\
&= -4x^{3} y^{-4} z^{-1} \\
&= -4 \frac{x^{3} y^{-4}}{x^{3} y^{-4}} \\
&= -4
\end{array}
$$



(b)

$$
\begin{array}{ll}
El_x z &= \frac{x}{z} \frac{\partial z}{\partial x} \\
&= \frac{x}{z} (2x \frac{1}{x^2 + y^2}) \\
&= \frac{2x^2}{(x^2 + y^2) \ln (x^2 + y^2)}
\end{array}
$$

$$
\begin{array}{ll}
El_y z &= \frac{y}{z} \frac{\partial z}{\partial y} \\
&= \frac{y}{z} (2y \frac{1}{x^2 + y^2}) \\
&= \frac{2y^2}{(x^2 + y^2) \ln (x^2 + y^2)}
\end{array}
$$



(c)

$$
\begin{array}{ll}
El_x z &= \frac{x}{z} \frac{\partial z}{\partial x} \\
&= \frac{x}{z} (e^{x + y}) \\
&= \frac{x}{e^{x + y}} (e^{x + y}) \\
&= x
\end{array}
$$

$$
\begin{array}{ll}
El_y z &= \frac{y}{z} \frac{\partial z}{\partial y} \\
&= \frac{y}{z} (e^{x + y}) \\
&= \frac{y}{e^{x + y}} (e^{x + y}) \\
&= y
\end{array}
$$





(d)

$$
\begin{array}{ll}
El_x z &= \frac{x}{z} \frac{\partial z}{\partial x} \\
&= \frac{x}{z} (0.5(x^2 + y^2)^{-0.5} (2x) ) \\
&= x^2(x^2 + y^2)^{-0.5} (x^2 + y^2)^{-0.5} ) \\
&= \frac{x^2}{x^2 + y^2}
\end{array}
$$

$$
\begin{array}{ll}
El_y z &= \frac{y}{z} \frac{\partial z}{\partial y} \\
&= \frac{y}{z} (0.5(x^2 + y^2)^{-0.5} (2y)) \\
&= y^2(x^2 + y^2)^{-0.5} (x^2 + y^2)^{-0.5} \\
&= \frac{y^2}{x^2 + y^2}
\end{array}
$$